src/Lean/Meta/Tactic/Grind/Arith/Offset.lean
@@ -4,7 +4,7 @@ Released under Apache 2.0 license as described in the file LICENSE.
 Authors: Leonardo de Moura
 -/
 prelude
-import Lean.Meta.Tactic.Arith.Offset.Main
-import Lean.Meta.Tactic.Arith.Offset.Proof
-import Lean.Meta.Tactic.Arith.Offset.Util
-import Lean.Meta.Tactic.Arith.Offset.Types
+import Lean.Meta.Tactic.Grind.Arith.Offset.Main
+import Lean.Meta.Tactic.Grind.Arith.Offset.Proof
+import Lean.Meta.Tactic.Grind.Arith.Offset.Util
+import Lean.Meta.Tactic.Grind.Arith.Offset.Types
